modularize Set/Seq functions and axioms

array-contains.bpl
@@ -39,70 +39,70 @@ axiom (forall n: Invoc, s: SeqInvoc :: {Seq_elem(n, Seq_append(s, n))}
 
 // Sets of invocations
 type SetInvoc;
-const emptySet: SetInvoc;
+const Set_empty: SetInvoc;
 
-function elem(n: Invoc, s: SetInvoc) : bool;
+function Set_elem(n: Invoc, s: SetInvoc) : bool;
 
-function subset(s: SetInvoc, t: SetInvoc) : bool;
+function Set_subset(s: SetInvoc, t: SetInvoc) : bool;
 
-// emptySet is a subset of anything
-axiom (forall s: SetInvoc :: subset(emptySet, s));
+// Set_empty is a subset of anything
+axiom (forall s: SetInvoc :: Set_subset(Set_empty, s));
 
-// Nothing is an elem of emptySet
-axiom (forall n: Invoc :: !elem(n, emptySet));
+// Nothing is an elem of Set_empty
+axiom (forall n: Invoc :: !Set_elem(n, Set_empty));
 
 // subset is reflexive
-axiom (forall s: SetInvoc :: subset(s, s));
+axiom (forall s: SetInvoc :: Set_subset(s, s));
 
 // subset is transitive
-axiom (forall s, t, u: SetInvoc :: subset(s, t) && subset(t, u) ==> subset(s, u));
+axiom (forall s, t, u: SetInvoc :: Set_subset(s, t) && Set_subset(t, u) ==> Set_subset(s, u));
 
 // definition of subset in terms of elem
-axiom (forall s, t: SetInvoc :: (forall n: Invoc :: elem(n, s) ==> elem(n, t)) ==> subset(s, t));
+axiom (forall s, t: SetInvoc :: (forall n: Invoc :: Set_elem(n, s) ==> Set_elem(n, t)) ==> Set_subset(s, t));
 
-function union(s1: SetInvoc, s2: SetInvoc) returns (t: SetInvoc);
+function Set_union(s1: SetInvoc, s2: SetInvoc) returns (t: SetInvoc);
 
 // union is idempotent
-axiom (forall s: SetInvoc :: s == union(s, s));
+axiom (forall s: SetInvoc :: s == Set_union(s, s));
 
 // union is associative
-axiom (forall s, t: SetInvoc :: union(s, t) == union(t, s));
+axiom (forall s, t: SetInvoc :: Set_union(s, t) == Set_union(t, s));
 
 // union is monotonic w.r.t subset
-axiom (forall s, t1, t2: SetInvoc :: subset(t1, t2) ==> subset(union(s, t1), union(s, t2)));
+axiom (forall s, t1, t2: SetInvoc :: Set_subset(t1, t2) ==> Set_subset(Set_union(s, t1), Set_union(s, t2)));
 
-axiom (forall s, t1, t2: SetInvoc :: subset(t1, s) && subset(t2, s) ==> subset(union(t1, t2), s));
+axiom (forall s, t1, t2: SetInvoc :: Set_subset(t1, s) && Set_subset(t2, s) ==> Set_subset(Set_union(t1, t2), s));
 
 // relation between union and elem
-axiom (forall n: Invoc, s, s1, t: SetInvoc :: elem(n, s) && s1 == union(s, t) ==> elem(n, s1));
+axiom (forall n: Invoc, s, s1, t: SetInvoc :: Set_elem(n, s) && s1 == Set_union(s, t) ==> Set_elem(n, s1));
 
 // Calculate the union m[i] \cup ... \cup m[j-1]
 function unionRange(m: [int]SetInvoc, i: int, j: int) returns (s: SetInvoc);
 
-function setOfSeq(q: SeqInvoc) returns (s: SetInvoc);
+function Set_ofSeq(q: SeqInvoc) returns (s: SetInvoc);
 
-function add(s: SetInvoc, n: Invoc) returns (t: SetInvoc);
+function Set_add(s: SetInvoc, n: Invoc) returns (t: SetInvoc);
 
 // Relation between add and elem
-axiom (forall s: SetInvoc, n1, n2: Invoc :: elem(n1, add(s, n2))
-       ==> n1 == n2 || elem(n1, s));
-axiom (forall s: SetInvoc, n1, n2: Invoc :: elem(n1, s) ==> elem(n1, add(s, n2)));
+axiom (forall s: SetInvoc, n1, n2: Invoc :: Set_elem(n1, Set_add(s, n2))
+       ==> n1 == n2 || Set_elem(n1, s));
+axiom (forall s: SetInvoc, n1, n2: Invoc :: Set_elem(n1, s) ==> Set_elem(n1, Set_add(s, n2)));
 
 // Relation between union and elem
-axiom (forall s, t: SetInvoc, n1: Invoc :: elem(n1, union(s, t))
-       ==> elem(n1, s) || elem(n1, t));
+axiom (forall s, t: SetInvoc, n1: Invoc :: Set_elem(n1, Set_union(s, t))
+       ==> Set_elem(n1, s) || Set_elem(n1, t));
 
 // add preserves subset relation
-axiom (forall s, t: SetInvoc, n: Invoc :: subset(s, t) ==> subset(add(s, n), add(t, n)));
-axiom (forall s, t: SetInvoc, n: Invoc :: subset(s, t) ==> subset(s, add(t, n)));
+axiom (forall s, t: SetInvoc, n: Invoc :: Set_subset(s, t) ==> Set_subset(Set_add(s, n), Set_add(t, n)));
+axiom (forall s, t: SetInvoc, n: Invoc :: Set_subset(s, t) ==> Set_subset(s, Set_add(t, n)));
 
 // Relation between setOfSeq, add, and append
-axiom (forall q: SeqInvoc, n: Invoc :: setOfSeq(Seq_append(q, n)) == add(setOfSeq(q), n));
+axiom (forall q: SeqInvoc, n: Invoc :: Set_ofSeq(Seq_append(q, n)) == Set_add(Set_ofSeq(q), n));
 
 // Relation between unionRange, add, and append
 axiom (forall t: [int]SetInvoc, i, j, k: int, q: SeqInvoc, n: Invoc ::
-        unionRange(t, i, j) == setOfSeq(q) && i <= k && k < j
-        ==> unionRange(t[k := add(t[k], n)], i, j) == setOfSeq(Seq_append(q, n)));
+        unionRange(t, i, j) == Set_ofSeq(q) && i <= k && k < j
+        ==> unionRange(t[k := Set_add(t[k], n)], i, j) == Set_ofSeq(Seq_append(q, n)));
 
 // Add n to m[i], ..., m[j-1]
 function addRange(m: [int]SetInvoc, n: Invoc, i: int, j: int)
@@ -111,15 +111,15 @@ function addRange(m: [int]SetInvoc, n: Invoc, i: int, j: int)
 // The effect of addRange
 axiom (forall m, m1: [int]SetInvoc, n: Invoc, i: int, j: int, k: int ::
         m1 == addRange(m, n, i, j) && i <= k && k < j
-        ==> m1[k] == add(m[k], n));
+        ==> m1[k] == Set_add(m[k], n));
 axiom (forall m, m1: [int]SetInvoc, n: Invoc, i: int, j: int, k: int ::
         m1 == addRange(m, n, i, j) && !(i <= k && k < j)
         ==> m1[k] == m[k]);
 
 // What happens to unionRange and setOfSeq when you do an addRange
 axiom (forall t: [int]SetInvoc, i, j, i1, j1: int, q: SeqInvoc, n: Invoc ::
-        unionRange(t, i, j) == setOfSeq(q) && i <= i1 && i1 < j1 && j1 <= j ==>
-          unionRange(addRange(t, n, i1, j1), i, j) == setOfSeq(Seq_append(q, n)));
+        unionRange(t, i, j) == Set_ofSeq(q) && i <= i1 && i1 < j1 && j1 <= j ==>
+          unionRange(addRange(t, n, i1, j1), i, j) == Set_ofSeq(Seq_append(q, n)));
 
 
 // ---------- Axioms of the map ADT
@@ -134,19 +134,19 @@ function invoc_v(n: Invoc) : int;
 function restr(s: SetInvoc, k: int) returns (t: SetInvoc);
 
 // restr is a subset
-axiom (forall s: SetInvoc, k: int :: subset(restr(s, k), s));
+axiom (forall s: SetInvoc, k: int :: Set_subset(restr(s, k), s));
 
 // restr is monotonic w.r.t subset
-axiom (forall s, t: SetInvoc, k: int :: subset(s, t) ==> subset(restr(s, k), restr(t, k)));
+axiom (forall s, t: SetInvoc, k: int :: Set_subset(s, t) ==> Set_subset(restr(s, k), restr(t, k)));
 
 // Adding an invocation on k increases restr
-axiom (forall q: SeqInvoc, n: Invoc :: {restr(setOfSeq(Seq_append(q, n)), invoc_k(n))}
-        restr(setOfSeq(Seq_append(q, n)), invoc_k(n))
-          == add(restr(setOfSeq(q), invoc_k(n)), n));
+axiom (forall q: SeqInvoc, n: Invoc :: {restr(Set_ofSeq(Seq_append(q, n)), invoc_k(n))}
+        restr(Set_ofSeq(Seq_append(q, n)), invoc_k(n))
+          == Set_add(restr(Set_ofSeq(q), invoc_k(n)), n));
 
 // Adding invocations not on k preserves restr
 axiom (forall q: SeqInvoc, n: Invoc, k: int :: invoc_k(n) != k
-       ==> restr(setOfSeq(Seq_append(q, n)), k) == restr(setOfSeq(q), k));
+       ==> restr(Set_ofSeq(Seq_append(q, n)), k) == restr(Set_ofSeq(q), k));
 
 type AbsState = [int]int; // Abstract state
 
@@ -157,12 +157,12 @@ function state(vis: SetInvoc, lin: SeqInvoc) returns (m: AbsState);
 
 // The effect of appending an invocation on key k on state of k
 axiom (forall s1, s2: SetInvoc, q1, q2: SeqInvoc, n: Invoc ::
-       q2 == Seq_append(q1, n) && s2 == add(s1, n)
+       q2 == Seq_append(q1, n) && s2 == Set_add(s1, n)
        ==> (invoc_m(n) == put ==> state(s2, q2)[invoc_k(n)] == invoc_v(n)));
 
 // Appending a get/contains invocation does not change state
 axiom (forall s1, s2: SetInvoc, q1, q2: SeqInvoc, n: Invoc, k: int ::
-       q2 == Seq_append(q1, n) && s2 == add(s1, n)
+       q2 == Seq_append(q1, n) && s2 == Set_add(s1, n)
        && (invoc_m(n) == get || invoc_m(n) == contains)
        ==> state(s2, q2)[k] == state(s1, q1)[k]);
 
@@ -175,22 +175,22 @@ axiom (forall s: SetInvoc, q1: SeqInvoc, n: Invoc, k: int ::
 axiom (forall s: SetInvoc, q: SeqInvoc, k: int ::
         state(s, q)[k] == state(restr(s, k), q)[k]);
 axiom (forall q: SeqInvoc, k: int ::
-        state(setOfSeq(q), q)[k] == state(restr(setOfSeq(q), k), q)[k]);
+        state(Set_ofSeq(q), q)[k] == state(restr(Set_ofSeq(q), k), q)[k]);
 
 // Taking union with a restriction of a super-set means restrictions are same
 axiom (forall s0, s1, t: SetInvoc, k: int ::
-        s1 == union(s0, t) && subset(restr(s0, k), t) ==>
+        s1 == Set_union(s0, t) && Set_subset(restr(s0, k), t) ==>
           restr(s1, k) == restr(t, k)
 );
 
 // Union of disjoint keys means state comes from one of the two sets
-procedure {:layer 1} lemma_state_union(k: int, s, t: SetInvoc);
-  requires (forall n: Invoc :: elem(n, s) ==> invoc_k(n) < k);
-  requires (forall n: Invoc :: elem(n, t) ==> k <= invoc_k(n));
+procedure {:layer 1} lemma_state_Set_union(k: int, s, t: SetInvoc);
+  requires (forall n: Invoc :: Set_elem(n, s) ==> invoc_k(n) < k);
+  requires (forall n: Invoc :: Set_elem(n, t) ==> k <= invoc_k(n));
   ensures (forall i: int :: 0 <= i && i < k ==>
-    state(union(s, t), lin)[i] == state(s, lin)[i]);
+    state(Set_union(s, t), lin)[i] == state(s, lin)[i]);
   ensures (forall i: int :: k <= i && i < tabLen ==>
-    state(union(s, t), lin)[i] == state(t, lin)[i]);
+    state(Set_union(s, t), lin)[i] == state(t, lin)[i]);
 
 
 // ---------- Representation of execution and linearization
@@ -239,19 +239,19 @@ function {:inline} tableInv(table: [int]int, abs: AbsState, tabvis: [int]SetInvo
                             called: [Invoc]bool, returned: [Invoc]bool) : bool
 {
   abstracts(table, abs)
-  && unionRange(tabvis, 0, tabLen) == setOfSeq(lin)
+  && unionRange(tabvis, 0, tabLen) == Set_ofSeq(lin)
   && (forall i: int :: 0 <= i && i < tabLen ==> state(tabvis[i], lin)[i] == abs[i])
   && (forall i: int :: 0 <= i && i < tabLen ==>
-      state(tabvis[i], lin)[i] == state(restr(setOfSeq(lin), i), lin)[i])
-  && (forall i: int :: 0 <= i && i < tabLen ==> subset(restr(setOfSeq(lin), i), tabvis[i]))
-  && (forall i: int :: 0 <= i && i < tabLen ==> subset(tabvis[i], setOfSeq(lin)))
-  && (forall i: int, n: Invoc :: 0 <= i && i < tabLen && elem(n, tabvis[i])
+      state(tabvis[i], lin)[i] == state(restr(Set_ofSeq(lin), i), lin)[i])
+  && (forall i: int :: 0 <= i && i < tabLen ==> Set_subset(restr(Set_ofSeq(lin), i), tabvis[i]))
+  && (forall i: int :: 0 <= i && i < tabLen ==> Set_subset(tabvis[i], Set_ofSeq(lin)))
+  && (forall i: int, n: Invoc :: 0 <= i && i < tabLen && Set_elem(n, tabvis[i])
       ==> invoc_k(n) == i)
   // Used to infer that invocations don't modify vis after they've returned
   && (forall n1, n2 : Invoc :: called[n1] && hb(n2, n1) ==> returned[n2])
   // Sanity conditions on vis sets
-  && (forall n1, n2 : Invoc :: elem(n2, vis[n1]) ==> elem(n2, tabvis[invoc_k(n2)]))
-  && (forall n1, n2 : Invoc :: elem(n2, vis[n1]) ==> 0 <= invoc_k(n2) && invoc_k(n2) < tabLen)
+  && (forall n1, n2 : Invoc :: Set_elem(n2, vis[n1]) ==> Set_elem(n2, tabvis[invoc_k(n2)]))
+  && (forall n1, n2 : Invoc :: Set_elem(n2, vis[n1]) ==> 0 <= invoc_k(n2) && invoc_k(n2) < tabLen)
   // To establish precondition of intro_writeLin
   && (forall n: Invoc :: returned[n] ==> Seq_elem(n, lin))
 }
@@ -286,18 +286,18 @@ procedure {:yields} {:layer 0} {:refines "readTable_spec"} readTable(k: int)
 
 procedure {:layer 1} intro_add_tabvis(k: int, n: Invoc)
   // TODO why don't these follow from the body?
-  ensures {:layer 1} tabvis == old(tabvis)[k := add(old(tabvis)[k], n)];
+  ensures {:layer 1} tabvis == old(tabvis)[k := Set_add(old(tabvis)[k], n)];
   modifies tabvis;
 {
-  tabvis[k] := add(tabvis[k], n);
+  tabvis[k] := Set_add(tabvis[k], n);
 }
 
 procedure {:layer 1} intro_read_tabvis_range(i, j: int) returns (s: SetInvoc);
   ensures {:layer 1} s == unionRange(tabvis, i, j);
-  ensures {:layer 1} (forall n: Invoc, k: int :: elem(n, tabvis[k]) && i <= k && k < j ==> elem(n, s));
+  ensures {:layer 1} (forall n: Invoc, k: int :: Set_elem(n, tabvis[k]) && i <= k && k < j ==> Set_elem(n, s));
   // TODO show these
-  ensures {:layer 1} (forall n1: Invoc :: elem(n1, s) ==> elem(n1, tabvis[invoc_k(n1)]));
-  ensures {:layer 1} (forall n1: Invoc :: elem(n1, s)
+  ensures {:layer 1} (forall n1: Invoc :: Set_elem(n1, s) ==> Set_elem(n1, tabvis[invoc_k(n1)]));
+  ensures {:layer 1} (forall n1: Invoc :: Set_elem(n1, s)
     ==> i <= invoc_k(n1) && invoc_k(n1) < j);
 
 procedure {:layer 1} intro_read_tabvis(k: int) returns (s: SetInvoc)
@@ -363,7 +363,7 @@ procedure {:atomic} {:layer 2} put_spec(k: int, v: int)
   lin := Seq_append(lin, this);
   vis[this] := my_vis;
   // Put is complete
-  assume my_vis == setOfSeq(lin);
+  assume my_vis == Set_ofSeq(lin);
 
   // Put satisfies its functional spec
   abs[k] := v;
@@ -403,7 +403,7 @@ procedure {:atomic} {:layer 2} get_spec(k: int) returns (v: int)
   lin := Seq_append(lin, this);
   vis[this] := my_vis;
   // Get is complete -- TODO make predicate
-  assume my_vis == setOfSeq(lin);
+  assume my_vis == Set_ofSeq(lin);
 
   // Get satisfies its functional spec
   v := abs[k];
@@ -452,7 +452,7 @@ procedure {:atomic} {:layer 2} contains_spec(v: int)
   lin := Seq_append(lin, this);
   vis[this] := my_vis;
   // Contains is monotonic
-  assume (forall j: Invoc :: hb(j, this) ==> subset(vis[j], my_vis));
+  assume (forall j: Invoc :: hb(j, this) ==> Set_subset(vis[j], my_vis));
 
   // Contains satisfies its functional spec
   assume contains_func_spec(my_vis, lin, witness_k, v, res);
@@ -471,36 +471,36 @@ procedure {:yields} {:layer 1} {:refines "contains_spec"} contains(v: int)
   yield; assert {:layer 1} tableInv(table, abs, tabvis, lin, vis, tabLen, called, returned) && inProgress(called, returned, this);
 
   k := 0;
-  my_vis := emptySet;
+  my_vis := Set_empty;
 
   while (k < tabLen)
     invariant {:layer 1} 0 <= k && k <= tabLen;
     invariant {:layer 1} tableInv(table, abs, tabvis, lin, vis, tabLen, called, returned) && inProgress(called, returned, this);
     invariant {:layer 1} (forall i: int :: 0 <= i && i < k ==> state(my_vis, lin)[i] != v);
-    invariant {:layer 1} subset(my_vis, setOfSeq(lin));
-    invariant {:layer 1} (forall n1 : Invoc :: elem(n1, my_vis) ==> elem(n1, tabvis[invoc_k(n1)]));
-    invariant {:layer 1} (forall n1 : Invoc :: elem(n1, my_vis) ==> 0 <= invoc_k(n1) && invoc_k(n1) < k);
+    invariant {:layer 1} Set_subset(my_vis, Set_ofSeq(lin));
+    invariant {:layer 1} (forall n1 : Invoc :: Set_elem(n1, my_vis) ==> Set_elem(n1, tabvis[invoc_k(n1)]));
+    invariant {:layer 1} (forall n1 : Invoc :: Set_elem(n1, my_vis) ==> 0 <= invoc_k(n1) && invoc_k(n1) < k);
     invariant {:layer 1} (forall n1, n2: Invoc ::
-                          hb(n1, this) && elem(n2, vis[n1])
+                          hb(n1, this) && Set_elem(n2, vis[n1])
                           && 0 <= invoc_k(n2) && invoc_k(n2) < k
-                          ==> elem(n2, my_vis));
+                          ==> Set_elem(n2, my_vis));
   {
     // Read table[k] and add tabvis[k] to my_vis
     call tv := readTable(k);
 
     call my_vis1 := intro_read_tabvis(k);
-    call lemma_state_union(k, my_vis, my_vis1);
-    my_vis := union(my_vis, my_vis1);
+    call lemma_state_Set_union(k, my_vis, my_vis1);
+    my_vis := Set_union(my_vis, my_vis1);
 
     if (tv == v) {
       // Linearization point
       call my_vis1 := intro_read_tabvis_range(k+1, tabLen);
       assert {:layer 1} (forall n1, n2: Invoc ::
-                          hb(n1, this) && elem(n2, vis[n1])
+                          hb(n1, this) && Set_elem(n2, vis[n1])
                           && 0 <= invoc_k(n2) && invoc_k(n2) < k+1
-                          ==> elem(n2, my_vis));
-      call lemma_state_union(k+1, my_vis, my_vis1);
-      my_vis := union(my_vis, my_vis1);
+                          ==> Set_elem(n2, my_vis));
+      call lemma_state_Set_union(k+1, my_vis, my_vis1);
+      my_vis := Set_union(my_vis, my_vis1);
       call intro_write_vis(this, my_vis);
       call intro_add_tabvis(tabLen-1, this);
       call intro_writeLin(this);
@@ -517,19 +517,19 @@ procedure {:yields} {:layer 1} {:refines "contains_spec"} contains(v: int)
     k := k + 1;
     yield; assert {:layer 1} tableInv(table, abs, tabvis, lin, vis, tabLen, called, returned) && inProgress(called, returned, this)
       && (forall i: int :: 0 <= i && i < k ==> state(my_vis, lin)[i] != v)
-      && subset(my_vis, setOfSeq(lin))
-      && (forall n1 : Invoc :: elem(n1, my_vis) ==> elem(n1, tabvis[invoc_k(n1)]))
-      && (forall n1 : Invoc :: elem(n1, my_vis) ==> 0 <= invoc_k(n1) && invoc_k(n1) < k);
-      assert {:layer 1} (forall n1, n2: Invoc :: hb(n1, this) && elem(n2, vis[n1])
-         && 0 <= invoc_k(n2) && invoc_k(n2) < k ==> elem(n2, my_vis));
+      && Set_subset(my_vis, Set_ofSeq(lin))
+      && (forall n1 : Invoc :: Set_elem(n1, my_vis) ==> Set_elem(n1, tabvis[invoc_k(n1)]))
+      && (forall n1 : Invoc :: Set_elem(n1, my_vis) ==> 0 <= invoc_k(n1) && invoc_k(n1) < k);
+      assert {:layer 1} (forall n1, n2: Invoc :: hb(n1, this) && Set_elem(n2, vis[n1])
+         && 0 <= invoc_k(n2) && invoc_k(n2) < k ==> Set_elem(n2, my_vis));
   }
   yield; assert {:layer 1} tableInv(table, abs, tabvis, lin, vis, tabLen, called, returned) && inProgress(called, returned, this)
     && (forall i: int :: 0 <= i && i < tabLen ==> state(my_vis, lin)[i] != v)
-    && (forall n1 : Invoc :: elem(n1, my_vis) ==> elem(n1, tabvis[invoc_k(n1)]))
-    && (forall n1 : Invoc :: elem(n1, my_vis) ==> 0 <= invoc_k(n1) && invoc_k(n1) < tabLen)
-    && (forall n1, n2: Invoc :: hb(n1, this) && elem(n2, vis[n1])
+    && (forall n1 : Invoc :: Set_elem(n1, my_vis) ==> Set_elem(n1, tabvis[invoc_k(n1)]))
+    && (forall n1 : Invoc :: Set_elem(n1, my_vis) ==> 0 <= invoc_k(n1) && invoc_k(n1) < tabLen)
+    && (forall n1, n2: Invoc :: hb(n1, this) && Set_elem(n2, vis[n1])
                          && 0 <= invoc_k(n2) && invoc_k(n2) < k
-                         ==> elem(n2, my_vis));
+                         ==> Set_elem(n2, my_vis));
 
   // Linearization point
   call intro_write_vis(this, my_vis);
